continue

Superposition_Calculus/First_Order_Type_System.thy
@@ -2,7 +2,8 @@ theory First_Order_Type_System
   imports First_Order_Clause
 begin
 
-inductive has_type for \<F> \<V> where
+inductive has_type :: 
+  "('f \<Rightarrow> 'ty list \<times> 'ty) \<Rightarrow> ('v \<Rightarrow> 'ty) \<Rightarrow> ('f,'v) term \<Rightarrow> 'ty \<Rightarrow> bool" for \<F> \<V> where
   Var: "\<V> x = \<tau> \<Longrightarrow> has_type \<F> \<V> (Var x) \<tau>" |
   Fun: "\<F> f = (\<tau>s, \<tau>) \<Longrightarrow> 
     list_all2 (has_type \<F> \<V>) ts \<tau>s \<Longrightarrow>
@@ -30,6 +31,14 @@ definition well_typed_cls_set where
 
 definition well_typed_subst where
   "well_typed_subst \<F> \<V> \<sigma> \<longleftrightarrow> (\<forall>x. has_type \<F> \<V> (\<sigma> x) (\<V> x))"
+
+definition well_typed_subst' where
+  "well_typed_subst' \<F> \<V> \<sigma> \<longleftrightarrow> 
+    (\<forall>x. has_type \<F> \<V> (Var x) (\<V> x) \<longrightarrow> has_type \<F> \<V> (\<sigma> x) (\<V> x))"
+
+definition well_typed_unifier where
+  "well_typed_unifier \<F> \<V> t\<^sub>1 t\<^sub>2 \<upsilon> \<longleftrightarrow> 
+    (\<forall>\<tau>. has_type \<F> \<V> t\<^sub>1 \<tau> \<longrightarrow> has_type \<F> \<V> t\<^sub>2 \<tau> \<longrightarrow> (\<forall>x. has_type \<F> \<V> (\<upsilon> x) (\<V> x)))"
 
 lemma well_typed_cls_add_mset: 
   "well_typed_cls \<F> \<V> (add_mset L C) \<longleftrightarrow> well_typed_lit \<F> \<V> L \<and> well_typed_cls \<F> \<V> C"
@@ -132,6 +141,10 @@ lemma well_typed_subst_clause:
   unfolding well_typed_cls_def subst_clause_def
   by blast
 
+definition well_typed_imgu where
+  "well_typed_imgu \<F> \<V> \<sigma> terms \<equiv> 
+    term_subst.is_imgu \<sigma> terms \<and> well_typed_subst \<F> \<V> \<sigma>"
+
 lemma ctxt_apply_term_preserves_typing:
   assumes
     \<kappa>_type: "has_type \<F> \<V> \<kappa>\<langle>t\<rangle> \<tau>\<^sub>1" and
@@ -165,6 +178,306 @@ next
   qed
   thus ?case
     by simp
+qed
+
+lemma well_typed_subst'_Var: "well_typed_subst' \<F> \<V> Var"
+  unfolding well_typed_subst'_def
+  by simp
+
+value "foldr (\<lambda>(x, t) \<sigma>. \<sigma> \<odot> Var(x := t)) [(x, t)] Var"
+
+
+lemma Fun_arg_types:
+  assumes 
+    "has_type \<F> \<V> (Fun f fs) \<tau>" 
+    "has_type \<F> \<V> (Fun f gs) \<tau>" 
+  obtains \<tau>s where 
+    "\<F> f = (\<tau>s, \<tau>)" 
+    "list_all2 (has_type \<F> \<V>) fs \<tau>s"
+    "list_all2 (has_type \<F> \<V>) gs \<tau>s"
+  by (metis Pair_inject assms(1) assms(2) has_type.simps term.distinct(1) term.inject(2))
+
+lemma welltyped_zip_option:
+  assumes 
+    "has_type \<F> \<V> (Fun f ts) \<tau>" 
+    "has_type \<F> \<V> (Fun f ss) \<tau>" 
+    "zip_option ts ss = Some ds" 
+  shows 
+    "\<forall>(a, b) \<in> set ds. \<exists>\<tau>. has_type \<F> \<V> a \<tau> \<and> has_type \<F> \<V> b \<tau>"
+proof-
+
+  obtain \<tau>s where 
+    (*"\<F> f = (\<tau>s, \<tau>)" *)
+    "list_all2 (has_type \<F> \<V>) ts \<tau>s"
+    "list_all2 (has_type \<F> \<V>) ss \<tau>s"
+    using Fun_arg_types[OF assms(1, 2)].
+
+  with assms(3) show ?thesis
+  proof(induction ts ss arbitrary: \<tau>s ds rule: zip_induct)
+    case (Cons_Cons t ts s ss)
+    then obtain \<tau>' \<tau>s' where \<tau>s: "\<tau>s = \<tau>' # \<tau>s'"
+      by (meson list_all2_Cons1)
+
+    from Cons_Cons(2) 
+    obtain d' ds' where ds: "ds = d' # ds'"
+      by auto
+
+    
+    have "zip_option ts ss = Some ds'"
+      using Cons_Cons(2) 
+      unfolding ds
+      by fastforce
+
+    moreover have "list_all2 (has_type \<F> \<V>) ts \<tau>s'" 
+      using Cons_Cons.prems(2) \<tau>s by blast
+
+    moreover have "list_all2 (has_type \<F> \<V>) ss \<tau>s'"
+      using Cons_Cons.prems(3) \<tau>s by blast
+
+    ultimately have "\<forall>(t, s)\<in>set ds'. \<exists>\<tau>. has_type \<F> \<V> t \<tau> \<and> has_type \<F> \<V> s \<tau>"
+      using Cons_Cons.IH
+      by presburger
+
+    moreover have "\<exists>\<tau>. has_type \<F> \<V> t \<tau> \<and> has_type \<F> \<V> s \<tau>"
+      using Cons_Cons.prems(2) Cons_Cons.prems(3) \<tau>s by blast
+  
+    ultimately show ?case
+      using Cons_Cons.prems(1) ds
+      by fastforce
+  qed(auto)
+qed
+
+lemma welltyped_decompose':
+  assumes
+    "has_type \<F> \<V> (Fun f fs) \<tau>" 
+    "has_type \<F> \<V> (Fun f gs) \<tau>"
+    "decompose (Fun f fs) (Fun g gs) = Some ds"
+  shows "\<forall>(t, t') \<in> set ds. \<exists>\<tau>. has_type \<F> \<V> t \<tau> \<and> has_type \<F> \<V> t' \<tau>"
+  using assms welltyped_zip_option[OF assms(1,2)]
+  by force
+  
+lemma welltyped_decompose:
+  assumes
+    "has_type \<F> \<V> f \<tau>" 
+    "has_type \<F> \<V> g \<tau>"
+    "decompose f g = Some ds"
+  shows "\<forall>(t, t') \<in> set ds. \<exists>\<tau>. has_type \<F> \<V> t \<tau> \<and> has_type \<F> \<V> t' \<tau>"
+proof-
+
+  obtain f' fs gs where "f = Fun f' fs" "g = Fun f' gs"
+    using assms(3)
+    unfolding decompose_def
+    by (smt (z3) option.distinct(1) prod.simps(2) rel_option_None1 term.split_sels(2))
+
+  then show ?thesis
+    using assms welltyped_decompose'
+    by (metis (mono_tags, lifting))
+qed
+    
+
+lemma welltyped_unify:
+  assumes 
+    "unify es bs = Some unifier"
+    "\<forall>(t, t') \<in> set es. \<exists>\<tau>. has_type \<F> \<V> t \<tau> \<and> has_type \<F> \<V> t' \<tau>"
+    "well_typed_subst \<F> \<V> (subst_of bs)"
+  shows "well_typed_subst \<F> \<V> (subst_of unifier)"
+  using assms
+proof(induction es bs arbitrary: unifier rule: unify.induct)
+  case (1 bs)
+  then show ?case
+    by simp
+next
+  case (2 f ss g ts E bs)
+  then obtain \<tau> where \<tau>:
+    "has_type \<F> \<V> (Fun f ss) \<tau>" 
+    "has_type \<F> \<V> (Fun g ts) \<tau>"
+    by auto
+
+  obtain ds where ds: "decompose (Fun f ss) (Fun g ts) = Some ds"
+    using 2(2)
+    by(simp split: option.splits)
+
+  moreover then have "unify (ds @ E) bs = Some unifier"
+    using "2.prems"(1) by auto
+
+  moreover have "\<forall>(t, t')\<in>set (ds @ E). \<exists>\<tau>. has_type \<F> \<V> t \<tau> \<and> has_type \<F> \<V> t' \<tau>"
+    using welltyped_decompose[OF \<tau> ds] 2(3)
+    by fastforce
+   
+  ultimately show ?case 
+    using 2(1) 2(4)
+    by blast
+next
+  case (3 x t E bs)
+  show ?case
+  proof(cases "t = Var x")
+    case True
+    then show ?thesis 
+      using 3
+      by simp
+  next
+    case False
+    then have "unify (subst_list (subst x t) E) ((x, t) # bs) = Some unifier"
+      using 3
+      by(auto split: if_splits)
+
+    moreover have 
+      "\<forall>(t, t') \<in> set (subst_list (subst x t) E). \<exists>\<tau>. has_type \<F> \<V> t \<tau> \<and> has_type \<F> \<V> t' \<tau>"
+      using 3(4)
+      unfolding subst_def subst_list_def
+      apply auto
+      by (smt (verit) case_prodD fun_upd_other fun_upd_same has_type.Var right_uniqueD right_unique_has_type well_typed_subst_def well_typed_subst_term)
+
+    moreover have "well_typed_subst \<F> \<V> (subst_of ((x, t) # bs))"
+      using 3(5)
+      sorry
+      
+
+    ultimately show ?thesis 
+      using 3(2)[OF False _ ]  "3.prems"(1) False by force
+  qed
+next
+  case (4 v va x E bs)
+  then show ?case sorry
+qed
+  
+lemma welltyped_unify:
+  assumes "unify [(t\<^sub>1, t\<^sub>2)] [] = Some unifier"
+  shows "well_typed_unifier \<F> \<V> t\<^sub>1 t\<^sub>2 (subst_of unifier)"
+  using assms 
+proof(induction "[(t\<^sub>1, t\<^sub>2)]" "[]:: ('a \<times> ('b, 'a) Term.term) list" rule: unify.induct)
+  case (2 f ss g ts)
+  then show ?case
+    apply (auto split: option.splits)
+    sorry
+next
+  case (3 x)
+  then show ?case
+    apply(auto simp: has_type.Var well_typed_unifier_def split: if_splits)
+    sorry
+next
+  case (4 v va x)
+  then show ?case
+    apply(auto split: if_splits)
+    sorry
+qed
+(*  case 1
+  then show ?case
+    unfolding well_typed_unifier_def
+    using has_type.Var
+    by fastforce
+next
+  case 2
+  then show ?case
+    by(simp split: option.splits)
+next
+  case (3 x t E bs)
+  then show ?case 
+  proof(cases "t = Var x")
+    case True
+    moreover have "unify E [] = Some bs"
+      using 3(3)
+      unfolding True
+      by simp
+      
+    ultimately show ?thesis
+      using 3
+      by blast
+  next
+    case False
+    moreover then have "x \<notin> vars_term t"
+      using "3.prems"
+      by fastforce
+
+    moreover have "unify (subst_list (subst x t) E) [] = Some ((x, t) # bs)"
+      using 3(3)
+      apply(auto simp: False split: if_splits)
+    proof(induction rule: unify.induct)
+      case (1 bs)
+      then show ?case
+        apply auto
+        sorry
+    next
+      case (2 f ss g ts E bs)
+      then show ?case sorry
+    next
+      case (3 x t E bs)
+      then show ?case sorry
+    next
+      case (4 v va x E bs)
+      then show ?case sorry
+    qed
+     
+
+    ultimately show ?thesis 
+      using 3 
+      sorry
+  qed
+next
+  case (4 f ts x E bs)
+  then have "x \<notin> vars_term (Fun f ts)"
+    by force
+   
+  have "unify (subst_list (subst x (Fun f ts)) E) [] = Some ((x, Fun f ts) # bs)"
+    sorry
+
+  then show ?case
+    sorry
+qed*)
+  
+lemma welltyped_the_mgu: 
+  assumes
+    "the_mgu t\<^sub>1 t\<^sub>2 = \<mu>"
+  shows 
+   "well_typed_unifier \<F> \<V> t\<^sub>1 t\<^sub>2 \<mu>"
+  using assms welltyped_unify[of t\<^sub>1 t\<^sub>2 _ \<F> \<V>]
+  unfolding the_mgu_def mgu_def well_typed_unifier_def 
+  by(auto simp: has_type.Var split: option.splits)
+ 
+lemma welltyped_imgu_exists:
+  fixes \<upsilon> :: "('f, 'v) subst"
+  assumes 
+    unified: "term \<cdot>t \<upsilon> = term' \<cdot>t \<upsilon>"
+  obtains \<mu> :: "('f, 'v) subst"
+  where 
+    "\<upsilon> = \<mu> \<odot> \<upsilon>" 
+    "term_subst.is_imgu \<mu> {{term, term'}}"
+    "well_typed_unifier \<F> \<V> term term' \<mu>"
+proof
+  have finite_terms: "finite {term, term'}"
+    by simp
+
+  have "term_subst.is_unifiers (the_mgu term term') {{term, term'}}"
+    unfolding term_subst.is_unifiers_def
+    using the_mgu_is_unifier[OF the_mgu[OF unified, THEN conjunct1]]
+    by simp
+
+  moreover have
+    "\<And>\<sigma>. term_subst.is_unifiers \<sigma> {{term, term'}} \<Longrightarrow> \<sigma> = the_mgu term term' \<odot> \<sigma>"
+    unfolding term_subst.is_unifiers_def
+    using
+      term_subst.is_unifier_iff_if_finite[OF finite_terms]
+      the_mgu[of "term" _ term']
+    by blast
+
+  ultimately have is_imgu: "term_subst.is_imgu (the_mgu term term') {{term, term'}}"
+    unfolding term_subst.is_imgu_def
+    by blast
+
+  show "\<upsilon> = (the_mgu term term') \<odot> \<upsilon>" 
+    using the_mgu[OF unified]
+    by blast
+
+  show "term_subst.is_imgu (the_mgu term term') {{term, term'}}"
+    using is_imgu
+    by blast
+
+  obtain \<mu> where \<mu>: "the_mgu term term' = \<mu>"
+    using assms ex_mgu_if_subst_apply_term_eq_subst_apply_term by blast
+
+  show "well_typed_unifier \<F> \<V> term term' (the_mgu term term')"
+    using welltyped_the_mgu[OF \<mu>, of \<F> \<V>]
+    unfolding \<mu>.
 qed
 
 end
